verify/boogie/templates/await.bpl
@@ -1,7 +1,7 @@
 var #registers: int;
 
 procedure await(cond : AwaitOp)
-    modifies step, effects, ordering, atomic, last_load, last_store, #state, #registers;
+    modifies step, atomic, last_load, last_store, #state, #registers;
 
     ensures {:msg "satisfy await condition"}
         cond[#output, old(#input1)];
