verify/boogie/templates/test.bpl
@@ -11,7 +11,7 @@ procedure read(ret : RMWOp, load_order: OrderRelation)
     ensures {:msg "load order"}
         load_order[last_load, old(step), step, ordering, effects];
     ensures {:msg "correct output"} (
-            exists v : int :: effects[last_load][read(old(a0),v,true)] &&
+            exists v : int :: effects[last_load] == read(old(a0),v,true) &&
                 a0 == ret[v, old(a1), old(a2)]
         );
 {
@@ -22,7 +22,7 @@ procedure read(ret : RMWOp, load_order: OrderRelation)
     loop: 
         // two loop invariants, used in every loop
         assert step >= old(step); 
-        assert (forall i : int, e : Effect :: old(step) <= i && i < step && effects[i][e] ==> ! (e is write));
+        assert (forall i : int, e : Effect :: old(step) <= i && i < step && effects[i] == e ==> ! (e is write));
 
         call a0 := execute(lr(false, false, x5));
         call x6 := execute(add(a0, a1));
@@ -39,7 +39,7 @@ procedure rmw (op: RMWOp)
     ensures {:msg "if no write happened, the value from memory is already the result of operation"} (
         var address, input1, input2 := old(a0), old(a1), old(a2);
         no_writes(old(step), step, last_store) ==>
-            (exists a,v : int, vis : bool :: effects[last_load][read(a,v,vis)] && v == op[v, input1, input2])
+            (exists a,v : int, vis : bool :: effects[last_load] == read(a,v,vis) && v == op[v, input1, input2])
     );
     
     ensures {:msg "atomicity"}
@@ -49,8 +49,8 @@ procedure rmw (op: RMWOp)
     ensures {:msg "store produces write to correct address with correct value"}
         !no_writes(old(step), step, last_store) ==> (
             var address, input1, input2 := old(a0), old(a1), old(a2);
-            (exists a,v : int, vis : bool :: effects[last_load][read(a,v,vis)]
-                && effects[last_store][write(address, op[v, input1, input2])])
+            (exists a,v : int, vis : bool :: effects[last_load] == read(a,v,vis)
+                && effects[last_store] == write(address, op[v, input1, input2)])
         );
 {
     // assumption about parameters
@@ -60,7 +60,7 @@ procedure rmw (op: RMWOp)
     loop: 
         // two loop invariants, used in every loop
         assert step >= old(step); 
-        assert (forall i : int, e : Effect :: old(step) <= i && i < step && effects[i][e] ==> ! (e is write));
+        assert (forall i : int, e : Effect :: old(step) <= i && i < step && effects[i] == e ==> ! (e is write));
 
         call a0 := execute(lr(false, false, x5));
         call x6 := execute(add(a0, a1));
@@ -73,7 +73,7 @@ procedure write(store_order: OrderRelation)
     modifies step, effects, ordering, atomic, last_load, last_store, local_monitor, monitor_exclusive, a0, a1, a2, x5, x6;
     ensures {:msg "no other writes"}
         (forall i : StateIndex ::
-            old(step) <= i && i < step && (exists e : Effect :: effects[i][e] && (e is write))
+            old(step) <= i && i < step && (exists e : Effect :: effects[i] == e && (e is write))
                 ==> i == last_store);
     ensures {:msg "store ordering"}
         !no_writes(old(step), step, last_store) ==> (
@@ -88,7 +88,7 @@ procedure write(store_order: OrderRelation)
     loop: 
         // two loop invariants, used in every loop
         assert step >= old(step); 
-        assert (forall i : int, e : Effect :: old(step) <= i && i < step && effects[i][e] ==> ! (e is write));
+        assert (forall i : int, e : Effect :: old(step) <= i && i < step && effects[i] == e ==> ! (e is write));
 
         call a0 := execute(lr(false, false, x5));
         call x6 := execute(add(a0, a1));
